Foundation/Modal/Kripke/Hilbert/K.lean
@@ -6,18 +6,19 @@ import Foundation.Modal.Kripke.Filteration
 namespace LO.Modal
 
 open Kripke
+open Hilbert.Kripke
 
 namespace Hilbert.K
 
-instance Kripke.sound : Sound (Hilbert.K) FrameClass.all := inferInstance
+instance Kripke.sound : Sound (Hilbert.K) FrameClass.all := instSound_of_validates_axioms FrameClass.all.validates_axiomK
 
-instance : Entailment.Consistent (Hilbert.K) := Hilbert.consistent_of_FrameClass FrameClass.all (by simp)
+instance : Entailment.Consistent (Hilbert.K) := consistent_of_sound_frameclass FrameClass.all (by simp)
 
 instance : Kripke.Canonical (Hilbert.K) FrameClass.all := ⟨by trivial⟩
 
 instance Kripke.complete : Complete (Hilbert.K) FrameClass.all := inferInstance
 
-instance Kripke.complete_finite : Complete (Hilbert.K) (FiniteFrameClass.all) := ⟨by
+instance Kripke.complete_finite : Complete (Hilbert.K) (FrameClass.finite_all) := ⟨by
   intro φ hp;
   apply Kripke.complete.complete;
   intro F _ V x;
@@ -25,10 +26,10 @@ instance Kripke.complete_finite : Complete (Hilbert.K) (FiniteFrameClass.all) :=
   let FM := coarsestFilterationModel M ↑φ.subformulas;
 
   apply filteration FM (coarsestFilterationModel.filterOf) (by aesop) |>.mpr;
-  apply validOnModel_of_validOnFiniteFrameClass hp;
-  . tauto;
-  . apply FilterEqvQuotient.finite;
-    simp;
+  apply hp;
+  apply Frame.isFinite_iff _ |>.mpr
+  apply FilterEqvQuotient.finite;
+  simp;
 ⟩
 
 end Hilbert.K
