Foundation/Modal/Kripke/Hilbert/K4Point3.lean
@@ -1,37 +1,37 @@
 import Foundation.Modal.Kripke.AxiomWeakPoint3
-import Foundation.Modal.Kripke.Hilbert.K4
+import Foundation.Modal.Kripke.Hilbert.Geach
 
 namespace LO.Modal
 
 open Kripke
+open Hilbert.Kripke
 open Geachean
-
 
 abbrev Kripke.FrameClass.trans_weakConnected : FrameClass := { F | Transitive F ∧ WeakConnected F }
 
-namespace Kripke.FrameClass.trans_weakConfluent
-
-protected instance definability_Hilbert
-  : FrameClass.DefinedBy Kripke.FrameClass.trans_weakConnected Hilbert.K4Point3.axioms := by
-  rw [
-    (show Kripke.FrameClass.trans_weakConnected = FrameClass.trans ∩ FrameClass.weakConnected by rfl),
-    (show Hilbert.K4Point3.axioms = Hilbert.K4.axioms ∪ {Axioms.WeakPoint3 (.atom 0) (.atom 1)} by aesop)
-  ];
-  exact FrameClass.definedBy_inter FrameClass.trans (Hilbert.K4.axioms) FrameClass.weakConnected {Axioms.WeakPoint3 (.atom 0) (.atom 1)};
+namespace Kripke.FrameClass.trans_weakConnected
 
 @[simp]
 protected lemma nonempty : Kripke.FrameClass.trans_weakConnected.Nonempty := by
-  use whitepoint.toFrame;
+  use whitepoint;
   simp [Transitive, WeakConnected];
 
-end Kripke.FrameClass.trans_weakConfluent
+lemma validates_HilbertK4Point3 : Kripke.FrameClass.trans_weakConnected.Validates Hilbert.K4Point3.axioms := by
+  apply FrameClass.Validates.withAxiomK;
+  rintro F ⟨_, _⟩ _ (rfl | rfl);
+  . exact validate_AxiomFour_of_transitive $ by assumption;
+  . apply weakConnected_of_validate_WeakPoint3 $ by assumption;;
+
+end Kripke.FrameClass.trans_weakConnected
 
 
 namespace Hilbert.K4Point3
 
-instance Kripke.sound : Sound (Hilbert.K4Point3) Kripke.FrameClass.trans_weakConnected := inferInstance
+instance Kripke.sound : Sound (Hilbert.K4Point3) Kripke.FrameClass.trans_weakConnected :=
+  instSound_of_validates_axioms FrameClass.trans_weakConnected.validates_HilbertK4Point3
 
-instance Kripke.consistent : Entailment.Consistent (Hilbert.K4Point3) := Hilbert.consistent_of_FrameClass Kripke.FrameClass.trans_weakConnected (by simp)
+instance Kripke.consistent : Entailment.Consistent (Hilbert.K4Point3) :=
+  consistent_of_sound_frameclass FrameClass.trans_weakConnected (by simp)
 
 instance Kripke.canonical : Canonical (Hilbert.K4Point3) Kripke.FrameClass.trans_weakConnected := ⟨Canonical.transitive, Canonical.weakConnected⟩
 
