Foundation/Modal/Kripke/Hilbert/KD.lean
@@ -3,21 +3,42 @@ import Foundation.Modal.Kripke.Hilbert.Geach
 namespace LO.Modal
 
 open Kripke
+open Hilbert.Kripke
 open Geachean
 
-abbrev Kripke.FrameClass.serial : FrameClass := { F | Serial F }
+namespace Kripke.FrameClass
+
+protected abbrev serial : FrameClass := { F | Serial F }
+
+namespace serial
+
+lemma isMultiGeachean : FrameClass.serial = FrameClass.multiGeachean {⟨0, 0, 1, 1⟩} := by
+  ext F;
+  simp [Geachean.serial_def, MultiGeachean]
+
+@[simp]
+lemma nonempty : FrameClass.serial.Nonempty := by simp [isMultiGeachean]
+
+lemma validates_AxiomD : FrameClass.serial.ValidatesFormula (Axioms.D (.atom 0)) := by
+  rintro F F_serial _ rfl;
+  apply validate_AxiomD_of_serial $ by assumption
+
+lemma validates_HilbertKD : FrameClass.serial.Validates Hilbert.KD.axioms := by
+  apply FrameClass.Validates.withAxiomK;
+  apply validates_AxiomD;
+
+end serial
+
+end Kripke.FrameClass
+
 
 namespace Hilbert.KD
 
-instance Kripke.sound : Sound (Hilbert.KD) Kripke.FrameClass.serial := by
-  convert Hilbert.Geach.Kripke.sound (G := {⟨0, 0, 1, 1⟩});
-  . exact eq_Geach;
-  . unfold Kripke.FrameClass.serial FrameClass.multiGeachean MultiGeachean;
-    simp [Geachean.serial_def];
+instance Kripke.sound : Sound (Hilbert.KD) Kripke.FrameClass.serial :=
+  instSound_of_validates_axioms FrameClass.serial.validates_HilbertKD
 
-instance Kripke.consistent : Entailment.Consistent (Hilbert.KD) := by
-  convert Hilbert.Geach.Kripke.consistent (G := {⟨0, 0, 1, 1⟩});
-  exact eq_Geach;
+instance Kripke.consistent : Entailment.Consistent (Hilbert.KD) :=
+  consistent_of_sound_frameclass FrameClass.serial (by simp)
 
 instance Kripke.canonical : Canonical (Hilbert.KD) Kripke.FrameClass.serial := ⟨Canonical.serial⟩
 
