Foundation/Modal/Kripke/Hilbert/KT.lean
@@ -3,21 +3,41 @@ import Foundation.Modal.Kripke.Hilbert.Geach
 namespace LO.Modal
 
 open Kripke
+open Hilbert.Kripke
 open Geachean
 
-protected abbrev Kripke.FrameClass.refl : FrameClass := { F | Reflexive F }
+namespace Kripke.FrameClass
+
+protected abbrev refl : FrameClass := { F | Reflexive F }
+
+
+namespace refl
+
+lemma isMultiGeachean : FrameClass.refl = FrameClass.multiGeachean {⟨0, 0, 1, 0⟩} := by
+  ext F;
+  simp [Geachean.reflexive_def, MultiGeachean]
+
+@[simp]
+lemma nonempty : FrameClass.refl.Nonempty := by simp [refl.isMultiGeachean]
+
+lemma validates_AxiomT : FrameClass.refl.ValidatesFormula (Axioms.T (.atom 0)) := by
+  rintro F F_refl _ rfl;
+  apply validate_AxiomT_of_reflexive $ by assumption
+
+lemma validates_HilbertKT : FrameClass.refl.Validates Hilbert.KT.axioms := Validates.withAxiomK validates_AxiomT
+
+end refl
+
+end Kripke.FrameClass
+
 
 namespace Hilbert.KT
 
-instance Kripke.sound : Sound (Hilbert.KT) Kripke.FrameClass.refl := by
-  convert Hilbert.Geach.Kripke.sound (G := {⟨0, 0, 1, 0⟩});
-  . exact eq_Geach;
-  . unfold Kripke.FrameClass.refl FrameClass.multiGeachean MultiGeachean;
-    simp [Geachean.reflexive_def];
+instance Kripke.sound : Sound (Hilbert.KT) Kripke.FrameClass.refl :=
+  instSound_of_validates_axioms Kripke.FrameClass.refl.validates_HilbertKT
 
-instance Kripke.consistent : Entailment.Consistent (Hilbert.KT) := by
-  convert Hilbert.Geach.Kripke.consistent (G := {⟨0, 0, 1, 0⟩});
-  exact eq_Geach;
+instance Kripke.consistent : Entailment.Consistent (Hilbert.KT) :=
+  consistent_of_sound_frameclass Kripke.FrameClass.refl (by simp)
 
 instance Kripke.canonical : Canonical (Hilbert.KT) Kripke.FrameClass.refl := ⟨Canonical.reflexive⟩
 
