Foundation/Modal/Kripke/Hilbert/S4.lean
@@ -4,47 +4,57 @@ import Foundation.Modal.Kripke.Filteration
 namespace LO.Modal
 
 open Kripke
+open Hilbert.Kripke
 open Geachean
 
 abbrev Kripke.FrameClass.preorder : FrameClass := { F | Reflexive F ∧ Transitive F }
-abbrev Kripke.FiniteFrameClass.preorder : FiniteFrameClass := { F | Reflexive F.Rel ∧ Transitive F.Rel }
+abbrev Kripke.FrameClass.finite_preorder: FrameClass := { F | F.IsFinite ∧ Reflexive F.Rel ∧ Transitive F.Rel }
 
-instance : Kripke.FrameClass.preorder.DefinedBy Hilbert.S4.axioms := by
-  convert FrameClass.multiGeachean.definability' {⟨0, 0, 1, 0⟩, ⟨0, 2, 1, 0⟩};
-  . unfold Kripke.FrameClass.preorder FrameClass.multiGeachean MultiGeachean;
-    simp [Geachean.reflexive_def, Geachean.transitive_def];
-  . exact Hilbert.S4.eq_Geach;
+namespace Kripke.FrameClass.preorder
+
+lemma isMultiGeachean : FrameClass.preorder = FrameClass.multiGeachean {⟨0, 0, 1, 0⟩, ⟨0, 2, 1, 0⟩} := by
+  ext F;
+  simp [Geachean.reflexive_def, Geachean.transitive_def, MultiGeachean]
+
+@[simp]
+lemma nonempty : FrameClass.preorder.Nonempty := by simp [isMultiGeachean]
+
+lemma validates_HilbertS4 : Kripke.FrameClass.preorder.Validates Hilbert.S4.axioms := by
+  apply FrameClass.Validates.withAxiomK;
+  rintro F ⟨F_refl, F_trans⟩ φ (rfl | rfl);
+  . exact validate_AxiomT_of_reflexive F_refl;
+  . exact validate_AxiomFour_of_transitive F_trans;
+
+end Kripke.FrameClass.preorder
+
 
 namespace Hilbert.S4.Kripke
 
-instance sound : Sound (Hilbert.S4) Kripke.FrameClass.preorder := by
-  convert Hilbert.Geach.Kripke.sound (G := {⟨0, 0, 1, 0⟩, ⟨0, 2, 1, 0⟩});
-  exact eq_Geach;
-  . unfold Kripke.FrameClass.preorder FrameClass.multiGeachean MultiGeachean;
-    simp [Geachean.reflexive_def, Geachean.transitive_def];
+instance sound : Sound (Hilbert.S4) Kripke.FrameClass.preorder :=
+  instSound_of_validates_axioms Kripke.FrameClass.preorder.validates_HilbertS4
 
-instance consistent : Entailment.Consistent (Hilbert.S4) := by
-  convert Hilbert.Geach.Kripke.consistent (G := {⟨0, 0, 1, 0⟩, ⟨0, 2, 1, 0⟩});
-  exact eq_Geach;
+instance consistent : Entailment.Consistent (Hilbert.S4) :=
+  consistent_of_sound_frameclass Kripke.FrameClass.preorder (by simp)
 
 instance canonical : Canonical (Hilbert.S4) Kripke.FrameClass.preorder := ⟨⟨Canonical.reflexive, Canonical.transitive⟩⟩
 
 instance complete : Complete (Hilbert.S4) Kripke.FrameClass.preorder := inferInstance
 
 open finestFilterationTransitiveClosureModel in
-instance finiteComplete : Complete (Hilbert.S4) Kripke.FiniteFrameClass.preorder := ⟨by
+instance finiteComplete : Complete (Hilbert.S4) Kripke.FrameClass.finite_preorder := ⟨by
   intro φ hp;
   apply Kripke.complete.complete;
   intro F ⟨F_refl, F_trans⟩ V x;
   let M : Kripke.Model := ⟨F, V⟩;
   let FM := finestFilterationTransitiveClosureModel M φ.subformulas;
   apply filteration FM (finestFilterationTransitiveClosureModel.filterOf F_trans) (by aesop) |>.mpr;
-  apply validOnModel_of_validOnFiniteFrameClass hp;
-  . refine ⟨?_, ?_⟩;
-    . exact reflexive_of_transitive_reflexive (by apply F_trans) F_refl;
-    . exact transitive;
-  . apply FilterEqvQuotient.finite;
+  apply hp;
+  refine ⟨?_, ?_, ?_⟩;
+  . apply Frame.isFinite_iff _ |>.mpr
+    apply FilterEqvQuotient.finite;
     simp;
+  . exact reflexive_of_transitive_reflexive F_trans F_refl;
+  . exact finestFilterationTransitiveClosureModel.transitive;
 ⟩
 
 end Hilbert.S4.Kripke
