Foundation/Modal/Kripke/Hilbert/S4Point3.lean
@@ -4,32 +4,35 @@ import Foundation.Modal.Kripke.AxiomPoint3
 namespace LO.Modal
 
 open Kripke
+open Hilbert.Kripke
 open Geachean
 
 abbrev Kripke.FrameClass.connected_preorder : FrameClass := { F | Reflexive F ∧ Transitive F ∧ Connected F }
 
-namespace Kripke.ReflexiveTransitiveConnectedFrameClass
-
-instance : FrameClass.DefinedBy Kripke.FrameClass.connected_preorder Hilbert.S4Point3.axioms := by
-  rw [
-    (show Kripke.FrameClass.connected_preorder = FrameClass.preorder ∩ FrameClass.connected by aesop),
-    (show Hilbert.S4Point3.axioms = Hilbert.S4.axioms ∪ {Axioms.Point3 (.atom 0) (.atom 1)} by aesop)
-  ];
-  exact FrameClass.definedBy_inter FrameClass.preorder (Hilbert.S4.axioms) FrameClass.connected {Axioms.Point3 (.atom 0) (.atom 1)};
+namespace Kripke.FrameClass.connected_preorder
 
 @[simp]
 protected lemma nonempty : Kripke.FrameClass.connected_preorder.Nonempty := by
-  use whitepoint.toFrame;
+  use whitepoint;
   simp [Reflexive, Transitive, Connected];
 
-end Kripke.ReflexiveTransitiveConnectedFrameClass
+lemma validates_HilbertS4Point3 : Kripke.FrameClass.connected_preorder.Validates Hilbert.S4Point3.axioms := by
+  apply FrameClass.Validates.withAxiomK;
+  rintro F ⟨_, _, _⟩ _ (rfl | rfl | rfl);
+  . exact validate_AxiomT_of_reflexive $ by assumption
+  . exact validate_AxiomFour_of_transitive $ by assumption;
+  . exact validate_AxiomPoint3_of_connected $ by assumption;
+
+end Kripke.FrameClass.connected_preorder
 
 
 namespace Hilbert.S4Point3.Kripke
 
-instance sound : Sound (Hilbert.S4Point3) Kripke.FrameClass.connected_preorder := inferInstance
+instance sound : Sound (Hilbert.S4Point3) Kripke.FrameClass.connected_preorder :=
+  instSound_of_validates_axioms FrameClass.connected_preorder.validates_HilbertS4Point3
 
-instance consistent : Entailment.Consistent (Hilbert.S4Point3) := Hilbert.consistent_of_FrameClass Kripke.FrameClass.connected_preorder
+instance consistent : Entailment.Consistent (Hilbert.S4Point3) :=
+  consistent_of_sound_frameclass FrameClass.connected_preorder (by simp)
 
 instance canonical : Canonical (Hilbert.S4Point3) Kripke.FrameClass.connected_preorder :=
   ⟨⟨Canonical.reflexive, Canonical.transitive, Canonical.connected⟩⟩
