Foundation/Propositional/Kripke/Hilbert/KC.lean
@@ -5,15 +5,39 @@ import Foundation.Propositional.Kripke.Hilbert.Soundness
 namespace LO.Propositional
 
 open Kripke
+open Hilbert.Kripke
 open Formula.Kripke
+
+namespace Kripke.FrameClass
+
+protected abbrev confluent : FrameClass := { F | Confluent F }
+
+namespace confluent
+
+@[simp]
+instance nonempty : FrameClass.confluent.Nonempty := by
+  use whitepoint;
+  simp [Confluent];
+
+lemma validates_AxiomWLEM : FrameClass.confluent.ValidatesFormula (Axioms.WeakLEM (.atom 0)) := by
+  rintro F _ _ rfl;
+  apply validate_WeakLEM_of_confluent $ by assumption
+
+instance validate_HilbertKC : FrameClass.confluent.Validates (Hilbert.KC.axioms) := by
+  apply FrameClass.Validates.withAxiomEFQ;
+  apply validates_AxiomWLEM;
+
+end confluent
+
+end Kripke.FrameClass
+
 
 namespace Hilbert.KC.Kripke
 
-instance : FrameClass.confluent.DefinedBy (Hilbert.KC.axioms) := FrameClass.definedBy_with_axiomEFQ inferInstance
+instance sound : Sound Hilbert.KC FrameClass.confluent :=
+  instSound_of_validates_axioms FrameClass.confluent.validate_HilbertKC
 
-instance sound : Sound Hilbert.KC FrameClass.confluent := inferInstance
-
-instance consistent : Entailment.Consistent Hilbert.KC := Kripke.Hilbert.consistent_of_FrameClass FrameClass.confluent (by simp)
+instance consistent : Entailment.Consistent Hilbert.KC := consistent_of_sound_frameclass FrameClass.confluent (by simp)
 
 instance canonical : Canonical Hilbert.KC FrameClass.confluent := ⟨Canonical.confluent⟩
 
