Foundation/Modal/Kripke/Hilbert/GL/Tree.lean
@@ -12,27 +12,26 @@ namespace Kripke
 
 variable (F : Kripke.Frame) {φ : Formula _}
 
-lemma valid_on_FiniteTransitiveTreeClass_of_valid_on_TransitiveIrreflexiveFrameClass (h : FiniteFrameClass.trans_irrefl ⊧ φ)
+lemma valid_on_FiniteTransitiveTreeClass_of_valid_on_TransitiveIrreflexiveFrameClass (h : FrameClass.finite_trans_irrefl ⊧ φ)
   : ∀ F : Kripke.Frame, ∀ r, [F.IsFiniteTree r] → F ⊧ φ := by
-  intro T r hT;
-  apply @h (T.toFinite);
-  refine ⟨hT.rel_transitive, hT.rel_irreflexive⟩;
+  intro F r hT;
+  apply h;
+  refine ⟨inferInstance, hT.rel_transitive, hT.rel_irreflexive⟩;
 
 lemma satisfies_at_root_on_FiniteTransitiveTree (h : ∀ F : Kripke.Frame, ∀ r, [F.IsFiniteTree r] → F ⊧ φ)
   : ∀ M : Model, ∀ r, [M.IsFiniteTree r] → Satisfies M r φ := fun M r _ => h M.toFrame r M.Val r
 
 open Model Classical in
 lemma valid_on_TransitiveIrreflexiveFrameClass_of_satisfies_at_root_on_FiniteTransitiveTree
-  : (∀ M : Model, ∀ r : M.World, (Frame.IsFiniteTree M.toFrame r) → Satisfies M r φ) → FiniteFrameClass.trans_irrefl ⊧ φ := by
-  rintro H F ⟨F_trans, F_irrefl⟩ V r;
-  let M : Kripke.Model := ⟨F.toFrame, V⟩;
+  : (∀ M : Model, ∀ r : M.World, (Frame.IsFiniteTree M.toFrame r) → Satisfies M r φ) → FrameClass.finite_trans_irrefl ⊧ φ := by
+  rintro H F ⟨_, F_trans, F_irrefl⟩ V r;
+  let M : Kripke.Model := ⟨F, V⟩;
   have : Satisfies ((M↾r).mkTransTreeUnravelling pointGenerate.root) mkTransTreeUnravelling.root φ := H _ _ ?_;
   have : Satisfies (M↾r) pointGenerate.root φ := mkTransTreeUnravelling.pMorphism (M↾r) (Frame.pointGenerate.rel_trans F_trans) _
     |>.modal_equivalence _
     |>.mp this;
   exact pointGenerate.pMorphism.modal_equivalence _ |>.mp this;
-  . have := F.world_finite;
-    exact @Frame.mkTransTreeUnravelling.instIsTree (F := (M↾r).toFrame) _
+  . exact @Frame.mkTransTreeUnravelling.instIsTree (F := (M↾r).toFrame) _
       (by
         apply @Frame.isFinite_iff (M↾r).toFrame |>.mpr;
         apply Subtype.finite;
@@ -49,7 +48,7 @@ namespace Hilbert.GL.Kripke
 theorem iff_provable_satisfies_FiniteTransitiveTree : Hilbert.GL ⊢! φ ↔ (∀ M : Model, ∀ r, M.IsFiniteTree r → Satisfies M r φ) := by
   constructor;
   . intro h M;
-    have : FiniteFrameClass.trans_irrefl ⊧ φ := Kripke.finite_sound.sound h;
+    have : FrameClass.finite_trans_irrefl ⊧ φ := Kripke.finite_sound.sound h;
     have := valid_on_FiniteTransitiveTreeClass_of_valid_on_TransitiveIrreflexiveFrameClass this;
     exact satisfies_at_root_on_FiniteTransitiveTree this M;
   . intro h;
