Foundation/Modal/Kripke/Hilbert/Soundness.lean
@@ -7,20 +7,17 @@ open Formula
 open Kripke
 open Formula.Kripke
 
-namespace Kripke.Hilbert
+namespace Hilbert.Kripke
 
-variable {H : Hilbert ℕ} {Γ : Set (Formula ℕ)} {φ : Formula ℕ}
+variable {H : Hilbert ℕ} {Γ : Set (Formula ℕ)} {φ : Formula ℕ} {C : Kripke.FrameClass}
 
-section
-
-variable {C : Kripke.FrameClass}
-
-lemma soundness_of_FrameClass_definedBy_axiomInstances [defined : C.DefinedBy H.axiomInstances] : H ⊢! φ → C ⊧ φ := by
+lemma soundness_of_validates_axiomInstances (hV : C.Validates H.axiomInstances)
+  : H ⊢! φ → C ⊧ φ := by
   intro hφ F hF;
   induction hφ using Hilbert.Deduction.rec! with
   | maxm h =>
     obtain ⟨ψ, h, ⟨s, rfl⟩⟩ := h;
-    apply defined.defines F |>.mp hF (ψ⟦s⟧);
+    apply hV F hF (ψ⟦s⟧);
     use ψ;
     constructor;
     . assumption;
@@ -31,25 +28,17 @@ lemma soundness_of_FrameClass_definedBy_axiomInstances [defined : C.DefinedBy H.
   | imply₂ => exact ValidOnFrame.imply₂;
   | ec => exact ValidOnFrame.elimContra;
 
-instance [defs : C.DefinedBy H.axioms] : C.DefinedBy H.axiomInstances := ⟨by
-  intro F;
-  constructor;
-  . rintro hF φ ⟨ψ, hψ, ⟨s, rfl⟩⟩;
-    exact ValidOnFrame.subst $ defs.defines F |>.mp hF ψ hψ;
-  . intro h;
-    apply defs.defines F |>.mpr;
-    intro φ hφ;
-    apply h;
-    use φ;
-    constructor;
-    . assumption;
-    . use .id;
-      simp;
+lemma validates_axioms_of_validates_axiomInstances (hV : C.Validates H.axioms) : C.Validates H.axiomInstances := by
+  rintro F hF _ ⟨φ, hφ, ⟨s, rfl⟩⟩;
+  exact ValidOnFrame.subst $ hV F hF φ hφ;
+
+instance instSound_of_validates_axioms (hV : C.Validates H.axioms) : Sound H C := ⟨fun {_} =>
+  soundness_of_validates_axiomInstances (validates_axioms_of_validates_axiomInstances hV)
 ⟩
 
-instance [C.DefinedBy H.axioms] : Sound H C := ⟨fun {_} => soundness_of_FrameClass_definedBy_axiomInstances⟩
-
-lemma consistent_of_FrameClass (C : Kripke.FrameClass) (C_nonempty: C.Nonempty := by simp) [sound : Sound H C] : Entailment.Consistent H := by
+lemma consistent_of_sound_frameclass
+  (C : Kripke.FrameClass) (C_nonempty: C.Nonempty := by simp) [sound : Sound H C]
+  : Entailment.Consistent H := by
   apply Entailment.Consistent.of_unprovable (f := ⊥);
   apply not_imp_not.mpr sound.sound;
   apply Semantics.set_models_iff.not.mpr;
@@ -60,67 +49,6 @@ lemma consistent_of_FrameClass (C : Kripke.FrameClass) (C_nonempty: C.Nonempty :
   . assumption;
   . simp;
 
-lemma finite_sound_of_sound (sound : Sound H C) : Sound H ({ F | F ∈ C ∧ Finite F }) := ⟨by
-  rintro φ hφ F ⟨hF₁, _⟩;
-  exact sound.sound hφ hF₁;
-⟩
-
-end
-
-
-
-section
-
-variable {C : Kripke.FiniteFrameClass}
-
-lemma soundness_of_FiniteFrameClass_definedBy_axiomInstances [defined : C.DefinedBy H.axiomInstances] : H ⊢! φ → C ⊧ φ := by
-  rintro hφ F hF;
-  induction hφ using Hilbert.Deduction.rec! with
-  | maxm h =>
-    obtain ⟨ψ, h, ⟨s, rfl⟩⟩ := h;
-    apply defined.defines F |>.mp hF (ψ⟦s⟧);
-    use ψ;
-    constructor;
-    . assumption;
-    . use s;
-  | mdp ihpq ihp => exact ValidOnFrame.mdp ihpq ihp;
-  | nec ih => exact ValidOnFrame.nec ih;
-  | imply₁ => exact ValidOnFrame.imply₁;
-  | imply₂ => exact ValidOnFrame.imply₂;
-  | ec => exact ValidOnFrame.elimContra;
-
-instance [defs : C.DefinedBy H.axioms] : C.DefinedBy H.axiomInstances := ⟨by
-  intro F;
-  constructor;
-  . rintro hF φ ⟨ψ, hψ, ⟨s, rfl⟩⟩;
-    exact ValidOnFrame.subst $ defs.defines F |>.mp hF ψ hψ;
-  . intro h;
-    apply defs.defines F |>.mpr;
-    intro φ hφ;
-    apply h;
-    use φ;
-    constructor;
-    . assumption;
-    . use .id;
-      simp;
-⟩
-
-instance [C.DefinedBy H.axioms] : Sound H C := ⟨fun {_} => soundness_of_FiniteFrameClass_definedBy_axiomInstances⟩
-
-lemma consistent_of_FiniteFrameClass (C : Kripke.FiniteFrameClass) (C_nonempty: C.Nonempty := by simp) [sound : Sound H C] : Entailment.Consistent H := by
-  apply Entailment.Consistent.of_unprovable (f := ⊥);
-  apply not_imp_not.mpr sound.sound;
-  apply Semantics.set_models_iff.not.mpr;
-  push_neg;
-  obtain ⟨F, hF⟩ := C_nonempty;
-  use F;
-  constructor;
-  . assumption;
-  . simp;
-
-end
-
-
-end Kripke.Hilbert
+end Hilbert.Kripke
 
 end LO.Modal
