Foundation/Modal/Logic/Sublogic/Grz.lean
@@ -21,15 +21,15 @@ instance : ProperSublogic Logic.S4 Logic.Grz := ⟨S4_ssubset_Grz⟩
 lemma Grz_ssubset_S5Grz : Logic.Grz ⊂ Logic.S5Grz := by
   constructor;
   . exact Hilbert.weakerThan_of_dominate_axioms (by simp) |>.subset;
-  . suffices ∃ φ, Hilbert.S5Grz ⊢! φ ∧ ¬FiniteFrameClass.strict_preorder ⊧ φ by simpa [Grz.eq_ReflexiveTransitiveAntiSymmetricFiniteKripkeFrameClass_Logic];
+  . suffices ∃ φ, Hilbert.S5Grz ⊢! φ ∧ ¬FrameClass.finite_strict_preorder ⊧ φ by simpa [Grz.eq_ReflexiveTransitiveAntiSymmetricFiniteKripkeFrameClass_Logic];
     use Axioms.Five (.atom 0)
     constructor;
     . exact axiomFive!;
-    . apply Kripke.not_validOnFiniteFrameClass_of_exists_finiteFrame;
-      let F : FiniteFrame := ⟨Fin 2, λ x y => x ≤ y⟩;
+    . apply Kripke.not_validOnFrameClass_of_exists_frame;
+      let F : Frame := ⟨Fin 2, λ x y => x ≤ y⟩;
       use F;
       constructor;
-      . refine ⟨?_, ?_, ?_⟩;
+      . refine ⟨by tauto, ?_, ?_, ?_⟩;
         . simp [F, Reflexive];
         . simp [F, Transitive]; omega;
         . simp [F, AntiSymmetric]; omega;
