Foundation/Modal/ModalCompanion/Int.lean
@@ -104,29 +104,11 @@ lemma Logic.Grz.is_largestMC_of_Int : Logic.Grz = Logic.Int.largestMC := by
 instance : ModalCompanion Logic.Int Logic.Grz := by
   rw [Logic.Grz.is_largestMC_of_Int];
   exact Modal.instModalCompanion_of_largestMC_via_KripkeSemantics
-    (IC := Propositional.Kripke.FiniteFrameClass.all.toFrameClass)
-    (MC := Modal.Kripke.FiniteFrameClass.strict_preorder.toFrameClass)
-    (by
-      intro φ;
-      simp only [Propositional.Logic.eq_kripkeFiniteFrameClass_toFrameClas_logic];
-      constructor;
-      . apply Propositional.Hilbert.Int.Kripke.sound_finite.sound;
-      . apply Propositional.Hilbert.Int.Kripke.complete_finite.complete;
-    )
-    (by
-      rw [←Logic.Grz.is_largestMC_of_Int];
-      intro φ;
-      simp only [Modal.Logic.eq_kripkeFiniteFrameClass_toFrameClas_logic];
-      constructor;
-      . apply Modal.Hilbert.Grz.Kripke.finite_sound.sound;
-      . apply Modal.Hilbert.Grz.Kripke.complete.complete;
-    )
-    (by
-      rintro _ ⟨F, hF, rfl⟩;
-      use ({ World := F.World, Rel := F.Rel, world_finite := F.world_finite });
-      simp only [Set.mem_setOf_eq, and_true];
-      refine ⟨F.rel_refl, F.rel_trans, F.rel_antisymm⟩;
-    )
+    (IC := Propositional.Kripke.FrameClass.finite_all)
+    (MC := Modal.Kripke.FrameClass.finite_strict_preorder)
+    (by rw [Logic.Int.Kripke.eq_all_finite])
+    (by rw [←Logic.Grz.is_largestMC_of_Int, Modal.Logic.Grz.eq_ReflexiveTransitiveAntiSymmetricFiniteKripkeFrameClass_Logic])
+    (by rintro F ⟨_⟩; refine ⟨by tauto, F.rel_refl, F.rel_trans, F.rel_antisymm⟩)
 
 end Grz
 
